

Title

Solution to Problem 1: Loop Invariant

Computing Binomial Coefficient Using Pseudocode and Loop Invariant

1. Original Pseudocode

```
get_binomial(n, k):  
1  x ← 1  
2  for i ← 1 to k do  
3      x ← x · (n - i + 1)  
4      x ← x / i  
5  return x
```

2. Binomial Coefficient Formula

The binomial coefficient counts the number of ways to choose k elements from n elements without repetition:

$$\binom{n}{k} = \frac{n!}{k! (n - k)!}$$

a. Loop Invariant

Invariant: At the beginning of each iteration i ,

$$x = \frac{\prod_{j=1}^{i-1} (n - j + 1)}{(i - 1)!}$$

Interpretation: After $i - 1$ iterations, x equals the partial binomial coefficient:

$$x = \frac{n \cdot (n - 1) \cdots (n - i + 2)}{1 \cdot 2 \cdots (i - 1)}$$

b. Proof of Loop Invariant

- **Base Case:** Before the loop starts, $x = 1, i = 1$ Formula gives:

$$\frac{\prod_{j=1}^0 (n - j + 1)}{0!} = 1$$

Invariant holds.

- **Inductive Step:** Assume invariant holds at start of iteration i :

$$x = \frac{\prod_{j=1}^{i-1} (n - j + 1)}{(i - 1)!}$$

After lines 3 and 4:

$$x \leftarrow x \cdot (n - i + 1), \quad x \leftarrow x / i$$

So:

$$x = \frac{\prod_{j=1}^i (n - j + 1)}{i!}$$

Invariant holds for next iteration.

c. Correctness

After k iterations:

$$x = \frac{\prod_{j=1}^k (n - j + 1)}{k!} = \frac{n(n - 1) \cdots (n - k + 1)}{k!} = \binom{n}{k}$$

Thus, the algorithm returns the correct binomial coefficient.

d. Python One-Liners

Using `math.comb`:

```
import math
binomial = lambda n, k: math.comb(n, k)
```

Without `math.comb`:

```
from functools import reduce
binomial = lambda n, k: reduce(lambda a,b: a*b, range(n-k+1, n+1)) //
reduce(lambda a,b: a*b, range(1, k+1))
```

extra. Complexity & Efficiency

- **Time Complexity:** OK because the loop runs k times.
- **Space Complexity:** $O(1)$ since only a few variables are used.
- This algorithm avoids computing full factorials, making it efficient for large n and small k .